formal/SkLean/MetaTy.lean
@@ -1,3 +1,0 @@
-import SkLean.Ast2
-import SkLean.Typing2
-import Mathlib.Tactic
